Interop stub: Pass parameters on the stack in Low* when needed

src/arch/x64/interop/Interop_Printer.fst
@@ -35,11 +35,11 @@ let print_low_nat_ty = function
   | TUInt128 -> "nat128"
 
 let print_low_ty = function
-  | TBuffer ty -> "B.buffer UInt8.t"
+  | TBuffer ty -> "b8"
   | TBase ty -> print_low_nat_ty ty
 
 let rec print_low_args = function
-  | [] -> "ST unit"
+  | [] -> "Stack unit"
   | (a, ty)::q -> a ^ ":" ^ print_low_ty ty ^ " -> " ^ print_low_args q
 
 let rec print_low_args_and = function
@@ -86,24 +86,19 @@ let rec print_length_t = function
   | [] -> ""
   | a::q -> single_length_t a ^ print_length_t q
 
-let rec disjoint args =
+let namelist_of_args args =
+  let rec aux = function
+  | [] -> ""
+  | [a, _] -> a
+  | (a, _)::q -> a ^ ";" ^ aux q in
+  "[" ^ aux args ^ "]" 
+
+let disjoint args =
   let args = List.Tot.Base.filter is_buffer args in
-  let rec disjoint_aux = function
-  | [] | [_] -> ""
-  | (a, _)::q -> begin
-    let rec aux = function
-      | [] -> ""
-      | [(b, _)] -> "disjoint " ^ a ^ " " ^ b
-      | (b, _)::r -> "disjoint " ^ a ^ " " ^ b ^ " /\\" ^ aux r
-  in aux q ^ disjoint_aux q
-  end in disjoint_aux args
+  "locs_disjoint " ^ namelist_of_args args
 
-let supported os target args = 
+let enough_registers os target args = 
   List.Tot.Base.length args <= List.Tot.Base.length (calling_registers os target)
-
-let supported_func os target func =
-  let _, args = func in
-  supported os target args
 
 let reg_to_low = function
   | "rax" -> "Rax"
@@ -124,10 +119,19 @@ let reg_to_low = function
   | "r15" -> "R15"
   | _ -> "error"
 
-let print_low_calling_args os target (args:list arg{supported os target args}) =
-  let rec aux regs (args:list arg{List.Tot.Base.length args <= List.Tot.Base.length regs}) =
+// TODO
+let print_low_calling_stack (args:list arg) =
+  let rec aux (i:nat) (args:list arg) : Tot string (decreases %[args]) = match args with
+    | [] -> ""
+    | (a, TBase _)::q -> "  let mem = buffer_write #(TBase TUInt64) stack_b " ^ (string_of_int i) ^ " " ^ a ^ " mem in\n" ^ aux (i+1) q
+    | (a, TBuffer _)::q -> "  let mem = buffer_write #(TBase TUInt64) stack_b " ^ (string_of_int i) ^ " (addrs " ^ a ^ ") mem in\n" ^ aux (i+1) q
+  in aux 0 args
+
+let print_low_calling_args os target (args:list arg) =
+  let rec aux regs (args:list arg) =
   match regs, args with
-    | _, [] -> "    | _ -> init_regs r"
+    | [], q -> "    | _ -> init_regs r end in\n" ^ print_low_calling_stack q
+    | _, [] -> "    | _ -> init_regs r end in\n"
     | r1::rn, (a, ty)::q -> "    | " ^ (reg_to_low r1) ^ " -> " ^ 
       (if TBuffer? ty then "addr_" ^ a else a) ^ 
       "\n" ^ aux rn q
@@ -160,13 +164,14 @@ let print_lengths args =
  | a::q  -> print_length a ^ " /\\ " ^ aux q
  in aux (List.Tot.Base.filter is_buffer args)
 
-let create_state os target args =
-  "  let buffers = " ^ print_buffers_list args ^ " in\n" ^
+let create_state os target args stack stack_length =
+  "  let buffers = " ^ (if stack then "stack_b::" else "") ^ print_buffers_list args ^ " in\n" ^
   "  let (mem:mem) = {addrs = addrs; ptrs = buffers; hs = h0} in\n" ^
   generate_low_addrs args ^
+  (if stack then "  let addr_stack:nat64 = addrs stack_b + " ^ (string_of_int stack_length) ^ " in\n" else "") ^
   "  let regs = fun r -> begin match r with\n" ^
+  (if stack then "    | Rsp -> addr_stack\n" else "") ^
   (print_low_calling_args os target args) ^
-  " end in\n" ^
   "  let xmms = init_xmms in\n" ^
   "  let s0 = {ok = true; regs = regs; xmms = xmms; flags = 0; mem = mem} in\n" ^
   print_length_t args
@@ -177,9 +182,9 @@ let print_vale_bufferty = function
   | TUInt128 -> "buffer128"
 
 let print_vale_ty = function
-  | TUInt8 -> "uint8"
-  | TUInt64 -> "uint64"  
-  | TUInt128 -> "uint128"
+  | TUInt8 -> "nat8"
+  | TUInt64 -> "nat64"  
+  | TUInt128 -> "quad32"
 
 let print_vale_full_ty = function
   | TBase ty -> print_vale_ty ty
@@ -189,10 +194,23 @@ let rec print_args_vale_list = function
   | [] -> ""
   | (a,ty)::q -> "(" ^ a ^ ":" ^ print_vale_full_ty ty ^ ") " ^ print_args_vale_list q
 
-let translate_lowstar os target (func:func_ty{supported_func os target func}) =
+let translate_lowstar os target (func:func_ty) =
   let name, args = func in
-  let separator0 = if (List.Tot.Base.length (List.Tot.Base.filter is_buffer args) = 0) then "" else " /\\ " in
-  let separator1 = if (List.Tot.Base.length (List.Tot.Base.filter is_buffer args) <= 1) then "" else " /\\ " in  
+  let buffer_args = List.Tot.Base.filter is_buffer args in
+  let nbr_stack_args = List.Tot.Base.length args - 
+    List.Tot.Base.length (calling_registers os target) in
+  let length_stack = nbr_stack_args `op_Multiply` 8 in
+  let stack_needed = nbr_stack_args > 0 in
+  let fuel_value = string_of_int (List.Tot.Base.length buffer_args + 3) in
+  let implies_precond = if stack_needed then "B.length stack_b == " ^ string_of_int length_stack ^
+    " /\ live h0 stack_b /\ locs_disjoint " ^ (namelist_of_args (("stack_b",TBuffer TUInt64)::buffer_args)) ^ " /\ "
+  else "" in
+  let stack_precond memname = if stack_needed then
+    "/\ B.length stack_b == " ^ string_of_int length_stack ^
+    " /\ live " ^ memname ^ " stack_b /\ locs_disjoint " ^ (namelist_of_args (("stack_b",TBuffer TUInt64)::buffer_args))
+  else "" in
+  let separator0 = if (List.Tot.Base.length buffer_args = 0) then "" else " /\\ " in
+  let separator1 = if (List.Tot.Base.length buffer_args <= 1) then "" else " /\\ " in  
   "module Vale_" ^ name ^
   "\n\nopen X64.Machine_s\nopen X64.Memory_i\nopen X64.Vale.State_i\nopen X64.Vale.Decls_i\n\n" ^
   "val va_code_" ^ name ^ ": unit -> va_code\n\n" ^
@@ -208,11 +226,26 @@ let translate_lowstar os target (func:func_ty{supported_func os target func}) =
   "(ensures (fun (va_sM, va_fM) -> va_post va_b0 va_s0 va_sM va_fM " ^ (print_args_names args) ^ "))" ^
   "\n\n\n\n" ^
   "module " ^ name ^
-  "\n\nopen LowStar.Buffer\nmodule B = LowStar.Buffer\nopen FStar.HyperStack.ST\nmodule HS = FStar.HyperStack\nopen Interop\nopen Words_s\nopen Types_s\nopen X64.Machine_s\nopen X64.Memory_i_s\nopen X64.Vale.State_i\nopen X64.Vale.Decls_i\n#set-options \"--z3rlimit 40\"\n\n" ^
+  "\n\nopen LowStar.Buffer\nmodule B = LowStar.Buffer\nopen LowStar.Modifies\nmodule M = LowStar.Modifies\nopen LowStar.ModifiesPat\nopen FStar.HyperStack.ST\nmodule HS = FStar.HyperStack\nopen Interop\nopen Words_s\nopen Types_s\nopen X64.Machine_s\nopen X64.Memory_i_s\nopen X64.Vale.State_i\nopen X64.Vale.Decls_i\n#set-options \"--z3rlimit 40\"\n\n" ^
   "open Vale_" ^ name ^ "\n\n" ^
-  "assume val st_put (h:HS.mem) (p:HS.mem -> Type0) (f:(h0:HS.mem{p h0}) -> GTot HS.mem) : ST unit (fun h0 -> p h0 /\ h == h0) (fun h0 _ h1 -> h == h0 /\ f h == h1)\n\n" ^
+  "assume val st_put (h:HS.mem) (p:HS.mem -> Type0) (f:(h0:HS.mem{p h0}) -> GTot HS.mem) : Stack unit (fun h0 -> p h0 /\ h == h0) (fun h0 _ h1 -> h == h0 /\ f h == h1)\n\n" ^
+  "let b8 = B.buffer UInt8.t\n\n" ^
+  "//This lemma will be available in the next version of Low*\n" ^
+  "assume val buffers_disjoint (b1 b2:b8) : Lemma
+  (requires M.loc_disjoint (M.loc_buffer b1) (M.loc_buffer b2))
+  (ensures B.disjoint b1 b2)
+  [SMTPat (B.disjoint b1 b2)]\n\n" ^
   "//The map from buffers to addresses in the heap, that remains abstract\n" ^
   "assume val addrs: addr_map\n\n" ^  
+   "let rec loc_locs_disjoint_rec (l:b8) (ls:list b8) : Type0 =\n" ^
+   "  match ls with\n" ^
+   "  | [] -> True\n" ^
+   "  | h::t -> M.loc_disjoint (M.loc_buffer l) (M.loc_buffer h) /\ loc_locs_disjoint_rec l t\n\n" ^
+  "let rec locs_disjoint_rec (ls:list b8) : Type0 =\n"^
+  "  match ls with\n"^
+  "  | [] -> True\n" ^
+  "  | h::t -> loc_locs_disjoint_rec h t /\ locs_disjoint_rec t\n\n" ^
+  "unfold\nlet locs_disjoint (ls:list b8) : Type0 = normalize (locs_disjoint_rec ls)\n\n" ^
   "// TODO: Complete with your pre- and post-conditions\n" ^
   "let pre_cond (h:HS.mem) " ^ (print_args_list args) ^ "= " ^ (liveness "h" args) ^ separator1 ^ (disjoint args) ^ separator0 ^ (print_lengths args) ^ "\n" ^
   "let post_cond (h0:HS.mem) (h1:HS.mem) " ^ (print_args_list args) ^ "= " 
@@ -220,16 +253,20 @@ let translate_lowstar os target (func:func_ty{supported_func os target func}) =
   "//The initial registers and xmms\n" ^
   "assume val init_regs:reg -> nat64\n" ^
   "assume val init_xmms:xmm -> quad32\n\n" ^
-  "#set-options \"--initial_fuel 4 --max_fuel 4 --initial_ifuel 2 --max_ifuel 2\"\n" ^
+  "#set-options \"--initial_fuel " ^ fuel_value ^ " --max_fuel " ^ fuel_value ^ " --initial_ifuel 2 --max_ifuel 2\"\n" ^
   "// TODO: Prove these two lemmas if they are not proven automatically\n" ^
-  "let implies_pre (h0:HS.mem) " ^ (print_args_list args) ^ ": Lemma\n" ^
-  "  (requires pre_cond h0 " ^ (print_args_names args) ^ ")\n" ^
-  "  (ensures (\n" ^
-  (create_state os target args) ^ 
-  "  va_pre (va_code_" ^ name ^ " ()) s0 " ^ (print_args_names args) ^ ")) =\n" ^
+  "let implies_pre (h0:HS.mem) " ^ (print_args_list args) ^ 
+  (if stack_needed then " (stack_b:b8) " else "") ^
+  ": Lemma\n" ^
+  "  (requires pre_cond h0 " ^ (print_args_names args) ^ stack_precond "h0" ^ ")\n" ^
+  "  (ensures (\n" ^ implies_precond ^ "(" ^
+  (create_state os target args stack_needed length_stack) ^ 
+  "  va_pre (va_code_" ^ name ^ " ()) s0 " ^ (print_args_names args) ^ "))) =\n" ^
   print_length_t args ^ 
   "  ()\n\n" ^
-  "let implies_post (va_s0:va_state) (va_sM:va_state) (va_fM:va_fuel) " ^ (print_args_list args) ^ " : Lemma\n" ^
+  "let implies_post (va_s0:va_state) (va_sM:va_state) (va_fM:va_fuel) " ^ (print_args_list args) ^
+  (if stack_needed then " (stack_b:b8)" else "") ^
+  " : Lemma\n" ^
   "  (requires pre_cond va_s0.mem.hs " ^ (print_args_names args) ^ "/\\\n" ^
   "    va_post (va_code_" ^ name ^ " ()) va_s0 va_sM va_fM " ^ (print_args_names args) ^ ")\n" ^
   "  (ensures post_cond va_s0.mem.hs va_sM.mem.hs " ^ (print_args_names args) ^ ") =\n" ^
@@ -239,11 +276,15 @@ let translate_lowstar os target (func:func_ty{supported_func os target func}) =
   "\n\t(requires (fun h -> pre_cond h " ^ (print_args_names args) ^ "))\n\t" ^
   "(ensures (fun h0 _ h1 -> post_cond h0 h1 " ^ (print_args_names args) ^ "))\n\n" ^
   "val ghost_" ^ name ^ ": " ^ (print_low_args_and args) ^ 
+  (if stack_needed then " stack_b:b8 -> " else "") ^
     "(h0:HS.mem{pre_cond h0 " ^ (print_args_names args) ^ 
+    stack_precond "h0" ^
     "}) -> GTot (h1:HS.mem{post_cond h0 h1 " ^ (print_args_names args) ^ "})\n\n" ^
-  "let ghost_" ^ name ^ " " ^ (print_args_names args) ^ "h0 =\n" ^
-  (create_state os target args) ^
-  "  implies_pre h0 " ^ (print_args_names args) ^ ";\n" ^
+  "let ghost_" ^ name ^ " " ^ (print_args_names args) ^
+  (if stack_needed then "stack_b " else "") ^ "h0 =\n" ^
+  (create_state os target args stack_needed length_stack) ^
+  "  implies_pre h0 " ^ (print_args_names args) ^ 
+  (if stack_needed then "stack_b " else "") ^ ";\n" ^
   "  let s1, f1 = va_lemma_" ^ name ^ " (va_code_" ^ name ^ " ()) s0 " ^ print_args_names args ^ " in\n" ^
   "  // Ensures that the Vale execution was correct\n" ^
   "  assert(s1.ok);\n" ^
@@ -251,12 +292,16 @@ let translate_lowstar os target (func:func_ty{supported_func os target func}) =
   (print_low_callee_saved os target) ^
   "  // Ensures that va_code_" ^ name ^ " is actually Vale code, and that s1 is the result of executing this code\n" ^
   "  assert (va_ensure_total (va_code_" ^ name ^ " ()) s0 s1 f1);\n" ^
-  "  implies_post s0 s1 f1 " ^ (print_args_names args) ^ ";\n" ^
+  "  implies_post s0 s1 f1 " ^ (print_args_names args) ^ 
+  (if stack_needed then "stack_b " else "") ^ ";\n" ^
   "  s1.mem.hs\n\n" ^
   "let " ^ name ^ " " ^ (print_args_names args) ^ " =\n" ^
+  (if stack_needed then "  push_frame();\n" ^
+    "  let (stack_b:b8) = B.alloca (UInt8.uint_to_t 0) (UInt32.uint_to_t " ^ string_of_int length_stack ^ ") in\n"  else "") ^
   "  let h0 = get() in\n" ^
-  "  st_put h0 (fun h -> pre_cond h " ^ (print_args_names args) ^ ") (ghost_" ^ name ^ " " ^ (print_args_names args) ^ ")\n"
-
+  "  st_put h0 (fun h -> pre_cond h " ^ (print_args_names args) ^ stack_precond "h" ^ ") (ghost_" ^ name ^ " " ^ (print_args_names args) ^ 
+  (if stack_needed then "stack_b);\n  pop_frame()\n" else ")\n")
+  
 let print_vale_arg = function
   | (a, TBuffer ty) -> "ghost " ^ a ^ ":" ^ print_vale_bufferty ty
   | (a, TBase ty) -> a ^ ":" ^ print_vale_ty ty
@@ -275,9 +320,13 @@ let rec print_buff_readable = function
   | [] -> ""
   | (a, _)::q -> "        buffer_readable(mem, "^a^");\n" ^ print_buff_readable q
 
-let print_calling_args os target (args:list arg{supported os target args}) =
-  let rec aux regs (args:list arg{List.Tot.Base.length args <= List.Tot.Base.length regs}) =
+//TODO
+let print_vale_calling_stack (args:list arg) = ""
+
+let print_calling_args os target (args:list arg) =
+  let rec aux regs (args:list arg) =
   match regs, args with
+    | [], q -> print_vale_calling_stack q
     | _, [] -> ""
     | r1::rn, (a, _)::q -> "        " ^ r1 ^ " == buffer_addr(" ^ a ^ ");\n" ^ aux rn q
   in aux (calling_registers os target) args
@@ -288,15 +337,14 @@ let print_callee_saved os target =
     | a::q -> "        " ^ a ^ " == old(" ^ a ^ ");\n" ^ aux q
   in aux (callee_saved os target)
 
-let print_vale_reads os target (args: list arg{supported os target args}) =
-  let rec aux regs (args:list arg{List.Tot.Base.length args <= List.Tot.Base.length regs}) = 
-  match regs, args with
-    | _, [] -> "\n"
-    | a::q, _::r -> a ^ "; " ^ aux q r
-  in aux (calling_registers os target) args
-
-let translate_vale os target (func:func_ty{supported_func os target func}) =
+let translate_vale os target (func:func_ty) =
   let name, args = func in
+  let args = ("stack_b", TBuffer TUInt64)::args in
+  let buffer_args = List.Tot.Base.filter is_buffer args in
+  let nbr_stack_args = List.Tot.Base.length args - 
+    List.Tot.Base.length (calling_registers os target) in
+  let length_stack = nbr_stack_args `op_Multiply` 8 in
+  let stack_needed = nbr_stack_args > 0 in  
   "module Vale_" ^ name ^
   "\n#verbatim{:interface}{:implementation}\n" ^ 
   "\nopen X64.Machine_s\nopen X64.Memory_i_s\nopen X64.Vale.State_i\nopen X64.Vale.Decls_i\n#set-options \"--z3rlimit 20\"\n#endverbatim\n\n" ^
